TouhouFormal/ECL.lean
@@ -39,4 +39,5 @@ import TouhouFormal.ECL.Callback
 import TouhouFormal.ECL.Interrupt
 import TouhouFormal.ECL.Extension
 import TouhouFormal.ECL.ChildContext
+import TouhouFormal.ECL.Misc
 import TouhouFormal.ECL.Boss
